tutorial/proofs/t05_main/generated_spec.v
@@ -1,6 +1,5 @@
 From refinedc.typing Require Import typing.
 From refinedc.tutorial.t05_main Require Import generated_code.
-From refinedc.examples.latch Require Import latch_def.
 From refinedc.examples.spinlock Require Import spinlock_def.
 Set Default Proof Using "Type".
 
@@ -12,6 +11,51 @@ Section spec.
   (* Inlined code. *)
 
   Definition alloc_initialized := initialized "allocator_state" ().
+
+  (* Definition of type [latch]. *)
+  Definition latch_rec : ((iProp Σ) -d> typeO) → ((iProp Σ) -d> typeO) := (λ self P,
+    struct struct_latch [@{type}
+      (atomic_bool (bool_it) ((□ P)) (True))
+    ]
+  )%I.
+  Typeclasses Opaque latch_rec.
+
+  Global Instance latch_rec_ne : Contractive latch_rec.
+  Proof. solve_type_proper. Qed.
+
+  Definition latch : rtype := {|
+    rty_type := (iProp Σ);
+    rty r__ := fixp latch_rec r__
+  |}.
+
+  Lemma latch_unfold (P : (iProp Σ)):
+    (P @ latch)%I ≡@{type} (
+      struct struct_latch [@{type}
+        (atomic_bool (bool_it) ((□ P)) (True))
+      ]
+    )%I.
+  Proof. by rewrite {1}/with_refinement/=fixp_unfold. Qed.
+
+
+  Global Program Instance latch_rmovable : RMovable latch :=
+    {| rmovable patt__ := movable_eq _ _ (latch_unfold patt__) |}.
+  Next Obligation. solve_ty_layout_eq. Qed.
+
+  Global Instance latch_simplify_hyp_place_inst l_ β_ patt__:
+    SimplifyHypPlace l_ β_ (patt__ @ latch)%I (Some 100%N) :=
+    λ T, i2p (simplify_hyp_place_eq l_ β_ _ _ T (latch_unfold _)).
+  Global Instance latch_simplify_goal_place_inst l_ β_ patt__:
+    SimplifyGoalPlace l_ β_ (patt__ @ latch)%I (Some 100%N) :=
+    λ T, i2p (simplify_goal_place_eq l_ β_ _ _ T (latch_unfold _)).
+
+  Global Program Instance latch_simplify_hyp_val_inst v_ patt__:
+    SimplifyHypVal v_ (patt__ @ latch)%I (Some 100%N) :=
+    λ T, i2p (simplify_hyp_val_eq v_ _ _ (latch_unfold _) T _).
+  Next Obligation. done. Qed.
+  Global Program Instance latch_simplify_goal_val_inst v_ patt__:
+    SimplifyGoalVal v_ (patt__ @ latch)%I (Some 100%N) :=
+    λ T, i2p (simplify_goal_val_eq v_ _ _ (latch_unfold _) T _).
+  Next Obligation. done. Qed.
 
   (* Definition of type [alloc_entry_t]. *)
   Definition alloc_entry_t_rec : ((list nat) -d> typeO) → ((list nat) -d> typeO) := (λ self sizes,
@@ -137,13 +181,13 @@ Section spec.
 
   (* Specifications for function [latch_wait]. *)
   Definition type_of_latch_wait :=
-    fn(∀ (p, beta, P) : loc * own_state * (iProp Σ); (p @ (&frac{beta} (latch (P)))); True)
-      → ∃ () : (), (void); (p ◁ₗ{beta} (latch (P))) ∗ (P).
+    fn(∀ (p, beta, P) : loc * own_state * (iProp Σ); (p @ (&frac{beta} (P @ (latch)))); True)
+      → ∃ () : (), (void); (p ◁ₗ{beta} (P @ (latch))) ∗ (P).
 
   (* Specifications for function [latch_release]. *)
   Definition type_of_latch_release :=
-    fn(∀ (p, beta, P) : loc * own_state * (iProp Σ); (p @ (&frac{beta} (latch (P)))); (□ P))
-      → ∃ () : (), (void); (p ◁ₗ{beta} (latch (P))).
+    fn(∀ (p, beta, P) : loc * own_state * (iProp Σ); (p @ (&frac{beta} (P @ (latch)))); (□ P))
+      → ∃ () : (), (void); (p ◁ₗ{beta} (P @ (latch))).
 
   (* Specifications for function [test]. *)
   Definition type_of_test :=
@@ -200,5 +244,6 @@ Section spec.
       → ∃ () : (), (int (i32)); True.
 End spec.
 
+Typeclasses Opaque latch_rec.
 Typeclasses Opaque alloc_entry_t_rec.
 Typeclasses Opaque alloc_state_rec.
